\documentclass{article}

\usepackage[utf8]{inputenc}
\usepackage{enumitem}
\usepackage{float}
\usepackage{circuitikz}
\usepackage{todonotes}
\usepackage{amsmath}
\usepackage{tikz}
\usetikzlibrary{shapes, calc, shapes, arrows}

\title{Blatt 3}
\author{Luca Kr√ºger, Jonas Otto, Jonas Merkle (Gruppe R)}
\date{\today}

\begin{document}
\maketitle

\section{Lernregeln}
$$E(w,b)=\frac{1}{2}\sum_{\mu=1}^{M}(T_{\mu}-f(wx_{\mu}+b))^2$$
\begin{enumerate}
  \item
        \begin{align*}
          \nabla E(w,b)=\begin{pmatrix} \dfrac{\strut \partial E}{\strut \partial w} \\ \dfrac{\strut \partial E}{\strut \partial b}\end{pmatrix} = \begin{pmatrix}
            - \sum_{\mu=1}^{M}(T_{\mu}-f(wx_{\mu}+b)) \cdot \dfrac{\strut \partial f(wx_{\mu}+b)}{\strut \partial w}\cdot x_{\mu} \\
            - \sum_{\mu=1}^{M}(T_{\mu}-f(wx_{\mu}+b)) \cdot \dfrac{\strut \partial f(wx_{\mu}+b)}{\strut \partial w}\end{pmatrix} \\
        \end{align*}
  \item
        \begin{enumerate}[label=\alph*)]
          \item inkrementelle Version:
                \begin{align*}
                  w(t+1) & =w(t)-\mu(T_{t}-f(wx_{t}+b)) \cdot \dfrac{\strut \partial f(wx_{t}+b)}{\strut \partial w}\cdot x_t \\
                  b(t+1) & =b(t)-\mu(T_{t}-f(wx_{t}+b)) \cdot \dfrac{\strut \partial f(wx_{t}+b)}{\strut \partial w}
                \end{align*}
          \item Batch Version
                \begin{align*}
                  w(t+1) & =w(t)+\mu\sum_{\mu=1}^{M}(T_{\mu}-f(wx_{\mu}+b)) \cdot \dfrac{\strut \partial f(wx_{\mu}+b)}{\strut \partial w}\cdot x_{\mu} \\
                  b(t+1) & =b(t)+\sum_{\mu=1}^{M}(T_{\mu}-f(wx_{\mu}+b)) \cdot \dfrac{\strut \partial f(wx_{\mu}+b)}{\strut \partial w}                 \\
                         & \text{mit}\ \mu \approx 1/M
                \end{align*}
        \end{enumerate}
  \item
\end{enumerate}



\end{document}
